modules/SMod2HMod.v
@@ -76,6 +76,9 @@ Section FSPEC.
   
 End FSPEC.
 
+Arguments precond: simpl never.
+Arguments postcond: simpl never.
+
 Section APC.
   Context `{Σ: GRA.t}.
   
@@ -248,22 +251,22 @@ Section HOARE.
 
 End HOARE.
 
-Module IPCNotations.
-  Notation ";;; t2" :=
-    (ITree.bind (trigger APC) (fun _ => t2))
-      (at level 63, t2 at next level, right associativity) : itree_scope.
-  Notation "` x : t <- t1 ;;; t2" :=
-    (ITree.bind t1 (fun x : t => ;;; t2))
-      (at level 62, t at next level, t1 at next level, x ident, right associativity) : itree_scope.
-  Notation "x <- t1 ;;; t2" :=
-    (ITree.bind t1 (fun x => ;;; t2))
-      (at level 62, t1 at next level, right associativity) : itree_scope.
-  Notation "' p <- t1 ;;; t2" :=
-    (ITree.bind t1 (fun x_ => match x_ with p => ;;; t2 end))
-      (at level 62, t1 at next level, p pattern, right associativity) : itree_scope.
-End IPCNotations.
+(* Module IPCNotations. *)
+  (* Notation ";;; t2" := *)
+  (*   (ITree.bind (trigger APC) (fun _ => t2)) *)
+  (*     (at level 63, t2 at next level, right associativity) : itree_scope. *)
+  (* Notation "` x : t <- t1 ;;; t2" := *)
+  (*   (ITree.bind t1 (fun x : t => ;;; t2)) *)
+  (*     (at level 62, t at next level, t1 at next level, x ident, right associativity) : itree_scope. *)
+  (* Notation "x <- t1 ;;; t2" := *)
+  (*   (ITree.bind t1 (fun x => ;;; t2)) *)
+  (*     (at level 62, t1 at next level, right associativity) : itree_scope. *)
+  (* Notation "' p <- t1 ;;; t2" := *)
+  (*   (ITree.bind t1 (fun x_ => match x_ with p => ;;; t2 end)) *)
+  (*     (at level 62, t1 at next level, p pattern, right associativity) : itree_scope. *)
+(* End IPCNotations. *)
 
-Export IPCNotations. 
+(* Export IPCNotations.  *)
 
 Module SModRed.
 Section RED.
